started with example

theories/module.v
@@ -1,12 +1,12 @@
 Require Import refframe.base.
 
-Inductive steps {A B} (R : A → list B → A → Prop) : A → list B → A → Prop :=
+Inductive steps {A B} (R : A → list B → A → Prop) : A → list (list B) → A → Prop :=
 | steps_refl ρ :
     steps R ρ [] ρ
 | steps_l ρ1 ρ2 ρ3 κ κs :
     R ρ1 κ ρ2 →
     steps R ρ2 κs ρ3 →
-    steps R ρ1 (κ ++ κs) ρ3.
+    steps R ρ1 (κ :: κs) ρ3.
 
 Record module := {
   m_state : Type;
@@ -21,12 +21,12 @@ Record module := {
 Definition safe (m : module) : Prop :=
   ∀ σ κ σ', m.(m_initial) σ → steps m.(m_step) σ κ σ' → m.(m_good) σ'.
 
-Record refines (mimpl mspec : module) (trans_initial : mimpl.(m_state) → mspec.(m_state)) (trans_event : mimpl.(m_event) → mspec.(m_event)) := {
+Record refines (mimpl mspec : module) (trans_initial : mimpl.(m_state) → mspec.(m_state)) (trans_event : list mimpl.(m_event) → list mspec.(m_event)) := {
   ref_initial σ : mimpl.(m_initial) σ → mspec.(m_initial) (trans_initial σ);
   ref_step σ κ σi:
-    safe mspec →
     mimpl.(m_initial) σ →
     steps mimpl.(m_step) σ κ σi →
+    (∀ σs, steps mspec.(m_step) (trans_initial σ) (trans_event <$> κ) σs → mspec.(m_good) σs) →
     mimpl.(m_good) σi ∧ ∃ σs, steps mspec.(m_step) (trans_initial σ) (trans_event <$> κ) σs;
 }.
 
@@ -34,7 +34,16 @@ Lemma refines_preserves_safe mspec mimpl ti te:
   safe mspec →
   refines mimpl mspec ti te →
   safe mimpl.
-Proof. move => Hs Hr σ κ σ' Hinit Hstep. by move: (ref_step _ _ _ _ Hr _ _ _ Hs Hinit Hstep) => [?[??]]. Qed.
+Proof.
+  move => Hs Hr σ κ σ' Hinit Hstep.
+  have [|]:= (ref_step _ _ _ _ Hr _ _ _ Hinit Hstep) => //.
+  move => σs Hsteps. apply: Hs => //.
+  by apply: ref_initial.
+Qed.
+
+Lemma refines_reflexive m:
+  refines m m id id.
+Proof. constructor => // σ κ σi Hi Hs. rewrite list_fmap_id. naive_solver. Qed.
 
 Lemma refines_vertical m1 m2 m3 ti1 te1 ti2 te2:
   refines m1 m2 ti1 te1 →
@@ -43,8 +52,163 @@ Lemma refines_vertical m1 m2 m3 ti1 te1 ti2 te2:
 Proof.
   move => Hr1 Hr2.
   constructor; first by destruct Hr1, Hr2; eauto.
-  move => σ κ σi Hsafe3 Hinit1 Hstep1 /=. rewrite list_fmap_compose.
-  have Hsafe2 := refines_preserves_safe _ _ _ _ Hsafe3 Hr2.
-  have [Hgood [σ2 Hstep2]] := (ref_step _ _ _ _ Hr1 _ _ _ Hsafe2 Hinit1 Hstep1). split => //.
-  have [|_ [σ3 Hstep3]] := (ref_step _ _ _ _ Hr2 _ _ _ Hsafe3 _ Hstep2); eauto using ref_initial.
+  move => σ κ σi Hinit1 Hstep1 /=. rewrite list_fmap_compose => Hsafe3.
+  have [|Hgood [σ2 Hstep2]] := (ref_step _ _ _ _ Hr1 _ _ _ Hinit1 Hstep1). {
+    move => σs2 Hstep2.
+    by have [||? _] := (ref_step _ _ _ _ Hr2 _ _ _ _ Hstep2); eauto using ref_initial.
+  }
+  split => //.
+  have [||_ [σ3 Hstep3]] := (ref_step _ _ _ _ Hr2 _ _ _ _ Hstep2); eauto using ref_initial.
 Qed.
+
+Inductive module_product_step (m1 m2 : module) : m1.(m_state) * m2.(m_state) → list (m1.(m_event) + m2.(m_event)) → m1.(m_state) * m2.(m_state) → Prop :=
+| ModuleStepBoth σ1 σ2 κs1 κs2 σ1' σ2' :
+    m1.(m_step) σ1 κs1 σ1' →
+    m2.(m_step) σ2 κs2 σ2' →
+    module_product_step m1 m2 (σ1, σ2) ((inl <$> κs1) ++ (inr <$> κs2)) (σ1', σ2)
+| ModuleStepLeft σ1 σ2 κs σ1' :
+    m1.(m_step) σ1 κs σ1' →
+    module_product_step m1 m2 (σ1, σ2) (inl <$> κs) (σ1', σ2)
+| ModuleStepRight σ1 σ2 κs σ2' :
+    m2.(m_step) σ2 κs σ2' →
+    module_product_step m1 m2 (σ1, σ2) (inr <$> κs) (σ1, σ2')
+.
+
+Definition module_product (m1 m2 : module) : module := {|
+  m_state := m1.(m_state) * m2.(m_state);
+  m_event := m1.(m_event) + m2.(m_event);
+  m_initial σ := m1.(m_initial) σ.1 ∧ m2.(m_initial) σ.2;
+  m_step := module_product_step m1 m2;
+  m_good σ := m1.(m_good) σ.1 ∧ m2.(m_good) σ.2;
+|}.
+
+
+
+
+
+
+(*
+  Example:
+                  High-level spec
+                  /------------\
+          --------              -------
+       Spec 1            +          Spec 2             Spec
+            |                         |
+            |                         |
+       Impl 1 High+ Memory High       |                  C
+            |           |             |
+            |           |             |
+       Impl 1 Low + Memory Low   +  Impl 2              ASM
+         --------      |       /------->
+                 \-----+-------
+        Low-level code including memory model (or without memory model?)
+
+
+
+  High-level spec:
+                           Res 1
+       Initial state  -------------->  Final State
+
+  Spec 1:                      Spec 2:
+                               (no main)
+   main: let x := Call A;       A: return 1
+         Emit (Res x)
+
+  Impl 1 High:                                    Memory High:
+
+   main: int* x = alloc_int;                      No offset operation on locations,
+         Call A x;                                Memory layout is hidden (i.e. integers are stored aso
+         Emit (Res *x)                            mathematical integers, constraint that all integers on the
+                                                  heap are 0 ≤ n < 2 ^ 32
+
+  Impl 1 Low:                  Impl 2 Low:        Memory Low:
+
+   main: int* x = alloc_int;   A p: *(p + 0) = 1; Flat memory model which stores bytes
+         Call A x;                  *(p + 1) = 0;
+         Emit (Res load_int(x))     *(p + 2) = 0;
+                                    *(p + 3) = 0;
+
+  Low level code (i.e. code with inline assembly)
+   main: int* x = alloc_int;     Flat memory model which stores bytes
+         *(x + 0) = 1;
+         *(x + 1) = 0;
+         *(x + 1) = 0;
+         *(x + 1) = 0;
+         Emit (Res load_int(x))
+
+
+ Proofs:
+
+  m1 < m2 : [refines m1 m2]
+  m1 + m2 : [module_product m1 m2]
+
+  1: LLC < Impl 1 Low + Memory Low + Impl 2
+
+  2: Impl 1 Low | Memory Low < Impl 1 High | Memory High
+
+  3: ∀ X1 X2,
+              calling convention change
+                     X1 < X2
+     ---------------------------------------------
+      Impl 1 High | Memory High | X1 < Spec 1 | Memory High | X2
+
+      calling convention change
+  4: Impl 2 | Memory Low < Spec 2
+
+  5: Spec 1 | Spec 2 < High-level Spec (HLS)
+
+  6: Memory Low < Memory High
+
+  Theorems:
+    Refl ([refines_reflexive]): m < m
+
+    VC ([refines_vertical]):     m1 < m2   m2 < m3
+                                 -----------------
+                                      m1 < m3
+
+    HC:       m1 < m1'   m2 < m2'
+             --------------------
+              m1 + m2 < m1' + m2'
+
+    | intro: (m1 | m2) + m2 < m1 + m2
+
+    | elim:   m1 + m2 < (m1 | m2) + m2
+
+    | ignore:       m1 < m2
+              ---------------------
+               (m1 | m) < (m2 | m)
+
+    +-I:            X m2          requires some condition X on m2
+              -----------------   something like none of its events appear in m3
+                m1 + m2 < m1
+
+    +-E:            X m2            requires some condition X on m2
+              -----------------     something like none of its events appear in m3
+                m1 < m1 + m2
+
+
+  Proof tree:
+
+   -------------------------------------- 1
+   LLC < Impl 1 Low + Memory Low + Impl 2
+   -------------------------------------------------------------------- VC, |-I
+   LLC < (Impl 1 Low | Memory Low | Impl 2) + Memory Low + (Impl 2 | Memory Low)
+   -------------------------------------------------------------------- HC, | ignore, 2, 4, 6
+   LLC < (Impl 1 High | Memory High | Impl 2) + Memory High + Spec 2
+   -------------------------------------------------------------------- HC, 3, 4
+   LLC < (Spec 1 | Memory High | Spec 2) + Memory High + Spec 2
+   ------------------------------------------------------------- VC,|-E
+   LLC < Spec 1 + Memory High + Spec 2
+                  |                                 ----------------------- 5
+                  |                                 (Spec 1 | Spec 2) < HLS
+                  |                                -------------------------------- VC, +-I
+                  |                                (Spec 1 | Spec 2) + Spec 2 < HLS
+    ------------------------------- VC,+-E         -------------------------------- VC, |-E
+    LLC < Spec 1 + Spec 2                           Spec 1 + Spec 2 < HLS
+   ------------------------------------------------ VC
+            LLC < HLS
+
+
+
+
+*)
